Completed an ntac proof of the infinitude of prime numbers. Added type semantic_tree and statement.

src/ntac/interactive.lean
@@ -1,9 +1,12 @@
 import ntac.ntac
-
+import tactic.ring
+import tactic.ring_exp
+import tactic.wlog
+import tactic.norm_num
 open tactic
 open interactive (parse)
-open tactic.interactive ( cases_arg_p propagate_tags)
-open interactive.types (texpr location using_ident with_ident_list only_flag)
+open tactic.interactive ( cases_arg_p rw_rules obtain_parse ring.mode)
+open interactive.types (texpr location using_ident with_ident_list only_flag ident_ pexpr_list_or_texpr)
 open lean.parser
 local postfix `?`:9001 := optional
 local postfix *:9001 := many
@@ -22,27 +25,33 @@ meta def getgoal1 : ntac expr :=
 do g::_ ← henkan get_goals,
 return g
 
-meta def getgoal1_or_done : ntac gost := 
+meta def getgoal1_or_done : ntac goal_tree := 
 do gs ← henkan get_goals,
 return $ match gs with
-| g::_ := gost.unres g
-| _ :=gost.done
+| g::_ := goal_tree.unres g
+| _ :=goal_tree.done
 end
 -- meta def exact (e : expr) (md := semireducible) : ntac unit := 
 -- do tg ← getgoal1,
 --    ret ← henkan $ tactic.exact e md,
 --    kata ← henkan (infer_type e),
---    replc_ntac tg (gost.exact e)
-meta def exact (e : expr) (md := semireducible) : ntac unit := 
-do tg ← getgoal1,
-   henkan $ tactic.exact e md
-
-meta def admit : ntac unit :=
-henkan target >>= exact ∘ expr.mk_sorry
-
+--    replc_ntac tg (goal_tree.exact e)
 meta def skiptgt : ntac unit :=
 do hg ← getgoal1,
-replc_ntac hg $ gost.skip $ gost.unres hg
+replc_ntac hg $ goal_tree.skip $ goal_tree.unres hg
+
+meta def exact (q : parse texpr) : ntac unit :=
+do tg ← getgoal1,
+tgt : expr ← henkan target,
+   e ← henkan $ i_to_expr_strict ``(%%q : %%tgt),
+   henkan $ tactic.exact e,
+   kata ← henkan (infer_type e),
+   replc_ntac tg (goal_tree.exact e)
+
+meta def «from» := exact
+meta def admit : ntac unit :=
+henkan $  target >>= tactic.exact ∘ expr.mk_sorry
+
 
 meta def «sorry» : ntac unit := admit
 
@@ -53,11 +62,11 @@ meta def induction (hp : parse cases_arg_p) (rec_name : parse using_ident) (ids 
 meta def aa : ntac unit :=
 fail "assumption tactic failed"
 
-meta def get_gost_expr_list (goals : list(name × expr)): ntac (list (gost × expr)) :=
+meta def get_goal_tree_expr_list (goals : list(name × expr)): ntac (list (goal_tree × expr)) :=
 do
 goal2 ← goals.mfilter $ λ ⟨n, m⟩, bnot <$> (henkan $ is_assigned m),
 goal2type ← henkan $ monad.sequence $ list.map (λ nex:name × expr, infer_type nex.2) goal2 ,
-let goal2unres := list.map (λ nex:name × expr, gost.unres $ nex.2) goal2 in
+let goal2unres := list.map (λ nex:name × expr, goal_tree.unres $ nex.2) goal2 in
 return $  list.zip goal2unres goal2type
 
 -- meta def assumption2 : ntac unit :=
@@ -74,7 +83,7 @@ let s := (do in_tag ← henkan get_main_tag,
       end) in
 mcond (henkan tags_enabled)
   s
-  (tac >> henkan skip)
+  (tac >> skip)
 
 meta def assumption : ntac unit :=
 do { ctx ← henkan local_context,
@@ -82,31 +91,59 @@ do { ctx ← henkan local_context,
      t   ← henkan target,
      H   ← henkan $ find_same_type t ctx,
      ty ← henkan $ infer_type H,
-     replc_ntac tg (gost.assumption t),--t janakute ty?
-     exact H}
+     replc_ntac tg (goal_tree.assumption t),--t janakute ty?
+     henkan $ tactic.exact H}
 <|> fail "assumption tactic failed"
 
-meta def rw (q : parse interactive.rw_rules) (l : parse location) (cfg : rewrite_cfg := {}) : ntac unit := do tg ← getgoal1, replc_ntac tg $ gost.rewrite $ gost.unres tg,henkan $ interactive.rw q l cfg
+meta def rw (q : parse interactive.rw_rules) (l : parse location) (cfg : rewrite_cfg := {}) : ntac unit := do tg ← getgoal1, replc_ntac tg $ goal_tree.rewrite $ goal_tree.unres tg,henkan $ interactive.rw q l cfg
 meta def delta (q : parse ident*) (l : parse location) (cfg : rewrite_cfg := {}) : ntac unit := henkan $ interactive.delta q l
 meta def simp (use_iota_eqn : parse $ (tk "!")?) (no_dflt : parse only_flag) (hs : parse simp_arg_list) (attr_names : parse with_ident_list)
               (locat : parse location) (cfg : simp_config_ext := {}) : ntac unit := 
               do tg ← getgoal1,
-               henkan $ interactive.simp use_iota_eqn no_dflt hs attr_names locat cfg,
-               ng ← getgoal1_or_done,
-               replc_ntac tg $ gost.simp ng
+              --(all_hyps, s, u) ← henkan $ mk_simp_set_core no_dflt attr_names hs tt,
+              --(hss, gex, hex, all_hyps) ← henkan $ decode_simp_arg_list_with_symm hs,
+              --gg ← henkan $ monad.sequence $ list.map (λ pe, tactic.to_expr pe tt ff) $ list.map prod.fst hss,
+              henkan $ interactive.simp use_iota_eqn no_dflt hs attr_names locat cfg,
+              ng ← getgoal1_or_done,
+              replc_ntac tg $ goal_tree.simp ng
+meta def simpa (use_iota_eqn : parse $ (tk "!")?) (no_dflt : parse only_flag)
+  (hs : parse simp_arg_list) (attr_names : parse with_ident_list)
+  (tgt : parse (tk "using" *> texpr)?) (cfg : simp_config_ext := {}) : ntac unit := henkan $ interactive.simpa use_iota_eqn no_dflt hs attr_names tgt cfg
 
-meta def apply (q : parse texpr) : ntac unit := 
+meta def rewrite (q : parse rw_rules) (l : parse location) (cfg : rewrite_cfg := {}) : ntac unit :=
+ do tg ← getgoal1,
+ henkan $ interactive.rewrite q l cfg,
+    ng ← getgoal1_or_done,
+    replc_ntac tg $ goal_tree.simp ng
+
+meta def rwa (q : parse rw_rules) (l : parse location) (cfg : rewrite_cfg := {}) : ntac unit :=
+rewrite q l cfg >> try assumption
+
+meta def apply_mycore (e : expr) (cfg : apply_cfg := {}) : ntac (list (name × expr)) := 
 do tg ← getgoal1,
-  h ← henkan $ i_to_expr_for_apply q,
-  goals ← henkan $ tactic.apply h,
-  glist ← get_gost_expr_list goals,
-  replc_ntac tg $ gost.apply h glist,
+  goals ← henkan $ tactic.apply e,
+  glist ← get_goal_tree_expr_list goals,
+  replc_ntac tg $ goal_tree.apply tg glist,
+  return goals
   --henkan $ interactive.concat_tags $ henkan2 $ return goals,
-  concat_tags $ return goals
 
+
+meta def apply  (q : parse texpr) : ntac unit :=
+concat_tags (do h ← henkan $ i_to_expr_for_apply q, apply_mycore h)
+meta def tact_eapply (e : expr) : ntac (list (name × expr)) :=
+apply_mycore e {new_goals := new_goals.non_dep_only}
+meta def eapply (q : parse texpr) : ntac unit :=
+concat_tags (henkan (i_to_expr_for_apply q) >>= tact_eapply)
+
+meta def by_cases : parse cases_arg_p → ntac unit
+| (n, q) := concat_tags $ do
+  p ← henkan $ tactic.to_expr_strict q,
+  henkan $ tactic.by_cases p (n.get_or_else `h),
+  pos_g :: neg_g :: rest ← henkan get_goals,
+  return [(`pos, pos_g), (`neg, neg_g)]
 
 meta def rsimp : ntac unit := do tg ← getgoal1, 
-henkan $ tactic.rsimp,tg2 ← getgoal1,replc_ntac tg $ gost.simp $ gost.unres tg2
+henkan $ tactic.rsimp,tg2 ← getgoal1,replc_ntac tg $ goal_tree.simp $ goal_tree.unres tg2
 
 
 @[inline] meta def readmy : ntac format :=
@@ -135,12 +172,154 @@ meta def trace_state2 : ntac unit := henkan tactic.interactive.trace_state
 meta def split : ntac unit :=
 do tg ← getgoal1,
 goals ← henkan $ tactic.split,
-glist ← get_gost_expr_list goals,
-let gost_new := gost.apply tg glist in 
-do replc_ntac tg gost_new,
+glist ← get_goal_tree_expr_list goals,
+let goal_tree_new := goal_tree.apply tg glist in 
+do replc_ntac tg goal_tree_new,
   concat_tags $ return goals
 
+meta def intro2_core (n : name) : ntac expr :=
+do tg ← getgoal1,
+ e ← henkan $ intro_core n,
+ te ← henkan $ infer_type e,
+ ng ← getgoal1,
+replc_ntac tg $ goal_tree.intro (n, te) $ goal_tree.unres ng,
+return e
 
+meta def intro2 (n : name) : ntac expr :=
+do t ← henkan target,
+   if expr.is_pi t ∨ expr.is_let t then intro2_core n
+   else henkan whnf_target >> intro2_core n
+
+meta def intro1 : ntac expr :=
+intro2 `_
+
+meta def focus1 {α} (tac : ntac α) : ntac α :=
+do g::gs ← henkan get_goals,
+   match gs with
+   | [] := tac
+   | _  := do
+      henkan $ set_goals [g],
+      a ← tac,
+      gs' ← henkan $ get_goals,
+      henkan $ set_goals (gs' ++ gs),
+      return a
+   end
+
+meta def propagate_tags (tac : ntac unit) : ntac unit :=
+do tag ← henkan get_main_tag,
+   if tag = [] then tac
+   else focus1 $ do
+     tac,
+     gs ← henkan get_goals,
+     when (bnot gs.empty) $ do
+       new_tag ← henkan get_main_tag,
+       when new_tag.empty $ henkan $ with_enable_tags (set_main_tag tag)
+
+meta def intro : parse ident_? → ntac unit
+| none     := propagate_tags (intro1 >> skip)
+| (some h) := propagate_tags (intro2 h >> skip)
+meta def rintro (p :parse rintro_parse ) : ntac unit := henkan $ interactive.rintro p
+meta def ring (red : parse (tk "!")?) (SOP : parse ring.mode) (loc : parse location) : ntac unit := henkan $ interactive.ring red SOP loc 
+meta def obtain  (p : parse obtain_parse ): ntac unit := henkan $ interactive.obtain p
+meta def use (l : parse pexpr_list_or_texpr) : ntac unit := henkan $ interactive.use l
+meta def rcases (p : parse rcases_parse ) : ntac unit := henkan $ interactive.rcases p
+meta def refine (q : parse texpr) : ntac unit :=
+henkan $ tactic.refine q
+
+meta def assert (h : name) (t : expr) : ntac expr :=
+do tg ← getgoal1,
+e ← henkan $ tactic.assert h t,
+tg1::tg2::_ ← henkan get_goals,
+replc_ntac tg $ goal_tree.willhave (goal_tree.unres tg1) (goal_tree.unres tg2), return e
+meta def assertv (h : name) (t : expr) (v : expr) : ntac expr :=
+do tg ← getgoal1,
+e ← henkan $ tactic.assertv h t v,
+tg1 ← getgoal1,
+replc_ntac tg $ goal_tree.have_ e (goal_tree.unres tg1), return e
+meta def note (h : name) (t : option expr := none) (pr : expr) : ntac expr :=
+do tg ← getgoal1,
+e ← henkan $ tactic.note h t pr,
+tg1 ← getgoal1,
+replc_ntac tg $ goal_tree.have_ e (goal_tree.unres tg1), return e
+meta def have_aux (h : parse ident?) (q₁ : parse (tk ":" *> texpr)?) (q₂ : parse $ (tk ":=" *> texpr)?) : ntac expr :=
+let h := h.get_or_else `this in
+match q₁, q₂ with
+| some e, some p := do
+  t ← henkan $ i_to_expr e,
+  v ←henkan $  i_to_expr ``(%%p : %%t),
+  assertv h t v
+| none, some p := do
+  p ←henkan $ i_to_expr p,
+  note h none p
+| some e, none := henkan (i_to_expr e) >>= assert h
+| none, none := do
+  u ←henkan $ mk_meta_univ,
+  e ← henkan $mk_meta_var (expr.sort u),
+  assert h e
+end
+meta def T : ntac unit :=
+do tg ← getgoal1,
+replc_ntac tg $ goal_tree.triv (goal_tree.unres tg)
+meta def «have» (h : parse ident?) (q₁ : parse (tk ":" *> texpr)?) (q₂ : parse $ (tk ":=" *> texpr)?) : ntac unit := 
+do e ← have_aux h q₁ q₂,
+skip
+
+
+meta def let_aux (h : parse ident?) (q₁ : parse (tk ":" *> texpr)?) (q₂ : parse $ (tk ":=" *> texpr)?) : ntac expr :=
+let h := h.get_or_else `this in
+henkan $ match q₁, q₂ with
+| some e, some p := do
+  t ← i_to_expr e,
+  v ← i_to_expr ``(%%p : %%t),
+  tactic.definev h t v
+| none, some p := do
+  p ← i_to_expr p,
+  tactic.pose h none p
+| some e, none := i_to_expr e >>= tactic.define h
+| none, none := do
+  u ← mk_meta_univ,
+  e ← mk_meta_var (expr.sort u),
+  tactic.define h e
+end
+meta def «let» (h : parse ident?) (q₁ : parse (tk ":" *> texpr)?) (q₂ : parse $ (tk ":=" *> texpr)?) : ntac unit :=
+do tg ← getgoal1,
+e ← let_aux h q₁ q₂,
+tg2 ← getgoal1,
+replc_ntac tg $ goal_tree.willhave (goal_tree.unres e) (goal_tree.unres tg2)
+
+private meta def target' : tactic expr :=
+target >>= instantiate_mvars >>= whnf
+
+private meta def apply_num_metavars : expr → expr → nat → tactic expr
+| f ftype 0     := return f
+| f ftype (n+1) := do
+  expr.pi m bi d b ← whnf ftype,
+  a          ← mk_meta_var d,
+  new_f      ← return $ f a,
+  new_ftype  ← return $ b.instantiate_var a,
+  apply_num_metavars new_f new_ftype n
+
+
+meta def existsi_org (e : expr) : ntac unit :=
+do tg ← getgoal1,
+[c]     ← henkan $ target' >>= get_constructors_for | fail "existsi tactic failed, target is not an inductive datatype with only one constructor",
+   fn      ← henkan $ mk_const c,
+   fn_type ← henkan $ infer_type fn,
+   n       ← henkan $  get_arity fn,
+   when (n < 2) (fail "existsi tactic failed, constructor must have at least two arguments"),
+   t       ← henkan $ apply_num_metavars fn fn_type (n - 2),
+   tact_eapply (expr.app t e),
+   t_type  ← henkan $ infer_type t >>= whnf,
+   e_type  ← henkan $ infer_type e,
+   (guard t_type.is_pi <|> fail "existsi tactic failed, failed to infer type"),
+   (henkan (unify t_type.binding_domain e_type) <|> fail "existsi tactic failed, type mismatch between given term witness and expected type"),
+   skip
+   --,replc_ntac tg $ goal_tree.existsi e $ goal_tree.unres tg
+
+
+meta def existsi : parse pexpr_list_or_texpr → ntac unit
+| []      := return ()
+| (p::ps) := henkan (i_to_expr p) >>= existsi_org >> existsi ps
 -- meta def seq'2 (tac1 : ntac unit) (tac2 : ntac unit) : ntac unit :=
 -- henkan1 "vovo" $ do g::gs ← get_goals,
 --    set_goals [g],
@@ -149,20 +328,29 @@ do replc_ntac tg gost_new,
 --    gs' ← get_goals,
 --    set_goals (gs' ++ gs)
 
+meta def by_contradiction (n : parse ident?) : ntac unit :=
+do tg ← getgoal1,
+henkan $ tactic.by_contradiction (n.get_or_else `h) $> (),
+tg2 ← getgoal1,
+replc_ntac tg $ goal_tree.contra (goal_tree.unres tg2)
+
+meta def by_contra (n : parse ident?) : ntac unit :=
+by_contradiction n
+
 meta def seq' (tac1 : ntac unit) (tac2 : ntac unit) : ntac unit :=
 do g::gs ← henkan get_goals,
-   gosts_bak ← get_gost,
+   goal_trees_bak ← get_goal_tree,
    henkan $ set_goals [g],
-   set_gost $ gost.unres g,
+   set_goal_tree $ goal_tree.unres g,
    tac1,
-   gosts ← get_gost,
+   goal_trees ← get_goal_tree,
    goals ← henkan get_goals,
-   set_gost $ let l := list.map (λ e, (e,gost.unres e)) goals in gost.andthen gosts l,
+   set_goal_tree $ let l := list.map (λ e, (e,goal_tree.unres e)) goals in goal_tree.andthen goal_trees l,
    all_goals' tac2,
-   gosts_new ← get_gost,
+   goal_trees_new ← get_goal_tree,
    gs' ← henkan get_goals,
    henkan $ set_goals (gs' ++ gs),
-   set_gost $ replc_unres g gosts_new gosts_bak
+   set_goal_tree $ replc_unres g goal_trees_new goal_trees_bak
 
 meta instance : has_andthen (ntac unit) (ntac unit) (ntac unit) :=
 ⟨seq'⟩
