src/myprime.lean
@@ -1,0 +1,38 @@
+import ntac
+import data.nat.prime
+
+open nat
+
+notation n `!`:10000 := nat.factorial n
+
+theorem exists_infinite_primes2 (n : ℕ) : ∃ p, n ≤ p ∧ prime p :=
+let p := min_fac (n! + 1) in
+have f1 : n! + 1 ≠ 1, from ne_of_gt $ succ_lt_succ $ factorial_pos _,
+have pp : prime p, from min_fac_prime f1,
+have np : n ≤ p, from le_of_not_ge $ λ h,
+  have h₁ : p ∣ n!, from dvd_factorial (min_fac_pos _) h,
+  have h₂ : p ∣ 1, from (nat.dvd_add_iff_right h₁).2 (min_fac_dvd _),
+  pp.not_dvd_one h₂,
+⟨p, np, pp⟩
+
+theorem exists_infinite_primes3 (n : ℕ) : ∃ p, n ≤ p ∧ prime p :=
+begin[ntac]
+let p := min_fac (n! + 1),trace_state,
+existsi p,trace_state,
+  have f1 : n! + 1 ≠ 1,
+  trace_state,
+  from (ne_of_gt $ succ_lt_succ $ factorial_pos n),
+  trace_state,
+  have pp : prime p, from min_fac_prime f1,
+split,
+{trace_state,
+  by_contradiction,trace_state,
+  simp at h,trace_state,
+  have h1: p ≤ n, from le_of_lt h,
+  have h₁ : p ∣ n!, from dvd_factorial (min_fac_pos _) h1,
+  have h₂ : p ∣ 1, from (nat.dvd_add_iff_right h₁).2 (min_fac_dvd _),
+  from  prime.not_dvd_one pp h₂,
+},
+T,{assumption}
+,trace_state
+end
