src/ntac/semantic_tree.lean
@@ -1,0 +1,20 @@
+inductive prop : Type
+| noun : prop
+
+meta inductive semantic_tree : Type
+| assume_prop : expr → semantic_tree → semantic_tree
+| assume_var : expr → semantic_tree → semantic_tree
+| but_false : semantic_tree → semantic_tree
+| assume_exist : expr → semantic_tree → semantic_tree
+| have_from : prop → prop → semantic_tree → semantic_tree
+| have_triv : prop → semantic_tree
+| suffice : prop → semantic_tree → semantic_tree
+| trivial : semantic_tree
+
+meta def semantic_tree_to_string : semantic_tree → string :=
+λ s,match s with
+| semantic_tree.trivial := "gtg"
+| semantic_tree.suffice p s := "dfdfd"
+| semantic_tree.have_from p v s := "df"
+| _ := "fg"
+  end
